src/deduction.lean
@@ -1,0 +1,80 @@
+import fopl
+
+universe u
+
+namespace language
+variables {L : language.{u}}
+
+def theory (L : language) := L.form → Prop
+
+inductive theory.sf (T : L.theory) : L.theory
+| intro : ∀ {p : L.form}, T p → theory.sf p.sf
+
+prefix `⇑`:max := theory.sf
+
+inductive provable : L.theory → L.form → Prop
+| gen : ∀ {T : theory L} {p}, provable (⇑T) p → provable T (Ȧp)
+| mp  : ∀ {T : theory L} {p q}, provable T (p →̇ q) → provable T p → provable T q
+| ax  : ∀ {T : theory L} {p}, T p → provable T p
+| p1  : ∀ (T : theory L) (p q), provable T (p →̇ q →̇ p)
+| p2  : ∀ (T : theory L) (p q r), provable T ((p →̇ q →̇ r) →̇ ((p →̇ q) →̇ (p →̇ r)))
+| p3  : ∀ (T : theory L) (p q), provable T ((¬̇ p →̇ ¬̇ q) →̇ (q →̇ p))
+| q1  : ∀ (T : theory L) (p t), provable T ((Ȧ p) →̇ p.(t))
+| q2  : ∀ (T : theory L) (p q), provable T ((Ȧ p →̇ q) →̇ (Ȧ p) →̇ Ȧ q)
+| q3  : ∀ (T : theory L) (p), provable T (p →̇ Ȧ p.sf)
+| e1  : ∀ (T : theory L) (t), provable T (t =̇ t)
+| e2  : ∀ (T : theory L) (p : L.form) (t u), provable T (t =̇ u →̇ p.(t) →̇ p.(u))
+
+infix ` ⊢̌ `:60 := provable
+
+attribute [simp] provable.p1 provable.p2 provable.p3 provable.q1 provable.q2 provable.q3
+  provable.e1 provable.e2
+
+def theory.consistent (T : L.theory) : Prop := ¬∃p, (T ⊢̌ p) ∧ (T ⊢̌ ¬̇p) 
+
+inductive theory.add (T : L.theory) (p : L.form) : L.theory 
+| new : theory.add p
+| old : ∀ {q}, T q → theory.add q
+
+infixl ` ¦ `:max := theory.add
+
+def theory.delete (T : L.theory) (p : L.form) : L.theory := λ q, T q ∧ q ≠ p
+
+def theory.include (T U : L.theory) : Prop := ∀ p, T p → U p
+
+instance : has_subset L.theory := ⟨theory.include⟩
+
+namespace provable
+variables (T : L.theory)
+
+@[simp] lemma pp (p) : T ⊢̌ p →̇ p :=
+by { have l₀ : T ⊢̌ (p →̇ (p →̇ p) →̇ p) →̇ (p →̇ p →̇ p) →̇ p →̇ p, simp,
+     have l₁ : T ⊢̌ p →̇ (p →̇ p) →̇ p, simp,
+     have l₂ : T ⊢̌ (p →̇ p →̇ p) →̇ p →̇ p, refine l₀.mp l₁,
+     have l₃ : T ⊢̌ p →̇ p →̇ p, simp,
+     refine l₂.mp l₃ }
+
+lemma imp_r {p} (h : T ⊢̌ p) (q) : T ⊢̌ q →̇ p :=
+by { have : T ⊢̌ p →̇ q →̇ p, simp,
+     exact this.mp h }
+
+variables {T}
+
+lemma inclusion {p} (h : T ⊢̌ p) : ∀ {U}, T ⊆ U → U ⊢̌ p :=
+begin
+  induction h with T p hyp_p IH T p q hyp_pq hyp_p IH₁ IH₂ T p hyp_p; try { simp },
+  { intros U hyp, refine gen (IH (λ x h, _)), cases h with p hp,
+    refine theory.sf.intro _, exact hyp _ hp },
+  { intros U hyp, exact (IH₁ hyp).mp (IH₂ hyp) },
+  { intros U hyp, exact ax (hyp _ hyp_p) }
+end
+
+lemma weakening (p) {q} : T ⊢̌ q → T ¦ p ⊢̌ q := λ hyp,
+inclusion hyp (λ x h, theory.add.old h)
+
+theorem deduction {p q} : T ¦ p ⊢̌ q → T ⊢̌ p →̇ q :=
+
+
+end provable
+
+end language
